Verbatim/memo/concrete_lexer.v
@@ -1,17 +1,288 @@
+Require Import List.
+Import ListNotations.
+
+Require Import Coq.ZArith.BinInt.
+
 From Verbatim Require Import regex.
 From Verbatim Require Import state.
-From Verbatim Require Import concrete_state.
-From Verbatim Require Import memo.
+From Verbatim Require Import lexer.abstraction.
+
+From Verbatim Require Import Table.
+From Verbatim Require Import DFA.
+From Verbatim Require Import lexer.impl.
+From Verbatim Require Import Utils.ltac.
+From Verbatim Require Import Utils.asciiFinite.
+From Verbatim Require Import Utils.ascii_order.
+From Verbatim Require Import concrete_table.
+
+From Verbatim Require Import memo.memo.
 From Verbatim Require Import memo.impl.
 From Verbatim Require Import memo.correctness.
 From Verbatim Require Import concrete_memo.
-From Verbatim Require Import lexer.abstraction.
 
 Module LexerFn (ALPHABET : SIGMA) (LABELS : LABEL).
 
-  Module Import R <: regex.T := regexTFn ALPHABET.
-  Module Import STT <: state.T := stateTFn R LABELS.
-  Module Import MEM <: memo.T := memoTFn STT.
+  Module Export MEM <: memo.T.
+    
+    Module Export STT <: state.T.
+      
+      Module TabT <: Table.T.
+        
+        Module Export R <: regex.T.
+          
+          Module Export Ty <: SIGMA := ALPHABET.
+          
+          Module Export Defs := regex.DefsFn Ty.
+          
+        End R.
+
+        Module TabTy <: TABLE R := FTable R.
+
+        Module Export Defs := DefsFn R TabTy.
+
+      End TabT.
+
+      Module Export R := TabT.R.
+      Import R.Ty.
+      Export R.Defs.Helpers.
+      
+      Module Export Ty <: STATE R.
+
+        Module Export D := DFAFn TabT. 
+
+        Definition Label : Type := LABELS.Label.
+        Definition defLabel : Label := LABELS.defLabel.
+        Lemma Label_eq_dec : forall (l l' : Label), {l = l'} + {l <> l'}.
+        Proof. apply LABELS.Label_eq_dec. Qed.
+        
+        Definition Pointer : Type := regex.
+        Definition defPointer : Pointer := EmptySet.
+        Definition Delta : Type := TabT.TabTy.Table * TabT.R.Defs.reFS.t.
+        Definition defDelta := (TabT.TabTy.emptyTable, TabT.TabTy.reFS.empty).
+        Definition State := prod Pointer Delta.
+        Definition defState := (defPointer, defDelta).
+        
+        Definition transition (a : Sigma) (e : State) : State :=
+          match e with
+            (x, (y, z)) =>
+            match DFAtransition a (x,y,z) with
+              (x',y',z') => (x',(y',z'))
+            end
+          end.
+        Definition transition_list (bs : list Sigma) (e : State) : State :=
+          match e with
+            (x, (y, z)) =>
+            match DFAtransition_list bs (x,y,z) with
+              (x',y',z') => (x',(y',z'))
+            end
+          end.
+        
+        Lemma transition_list_nil : forall fsm,
+            transition_list [] fsm = fsm.
+        Proof.
+          intros. unfold transition_list. repeat dm.
+        Qed.
+        
+        Lemma transition_list_cons : forall bs a fsm,
+            transition_list (a :: bs) fsm = transition_list bs (transition a fsm).
+        Proof.
+          intros. unfold transition_list. repeat dm. sis. repeat dm.
+          - repeat inj_all.
+            assert((r, t2, t1) = (r0, t6, t5)).
+            { rewrite <- E1. rewrite <- E5. auto. }
+            inv H. auto.
+          - repeat inj_all.
+            assert((r, t2, t1) = (r0, t6, t5)).
+            { rewrite <- E1. rewrite <- E5. auto. }
+            inv H. auto.
+        Qed.
+        
+        Lemma transition_Delta : forall a p p' d d',
+            transition a (p, d) = (p', d') -> d = d'.
+        Proof.
+          intros. unfold transition in *. repeat dm. repeat inj_all.
+          apply DFAtransition_Delta in E0. destruct E0. subst. auto.
+        Qed.
+        
+        Definition accepts (s : String) (e : State) : bool :=
+          match e with
+            (x, (y, z)) => DFAaccepts s (x, y, z)
+          end.
+        Definition accepting (e : State) :=
+          match e with
+            (x, (y, z)) => DFAaccepting (x, y, z)
+          end.
+
+        Lemma accepts_nil: forall(fsm : State), accepting fsm = accepts [] fsm.
+        Proof. intros fsm. reflexivity. Qed.
+
+        Lemma accepts_transition : forall cand a fsm,
+            accepts cand (transition a fsm) = accepts (a :: cand) fsm.
+        Proof.
+          intros. unfold accepts. repeat dm. rewrite accepts_cons. unfold transition in E.
+          repeat dm. repeat inj_all. auto.
+        Qed.
+
+        Definition init_state (r : regex) : State :=
+          match regex2dfa r with
+            (x, y, z) => (x, (y, z))
+          end.
+        Definition init_state_inv (r : State) : regex :=
+          match r with
+            (x, (y, z)) => dfa2regex (x, y, z)
+          end.
+        
+        Lemma invert_init_correct : forall r s,
+            exp_match s (init_state_inv (init_state r)) <-> exp_match s r.
+        Proof. intros. simpl. apply TabT.Defs.FillTable.canon_equiv. Qed.
+        
+        Lemma accepts_matches : forall(s : String) (e : regex),
+            true = accepts s (init_state e) <-> exp_match s e.
+        Proof.
+          split; intros.
+          - symmetry in H. apply r2d_accepts_match. auto.
+          - symmetry. apply r2d_accepts_match. auto.
+        Qed.
+
+        Definition accepting_dt_list : forall bs e,
+            accepting (transition_list bs (init_state e))
+            = accepting (init_state (derivative_list bs e)).
+        Proof.
+          intros. unfold accepting. repeat dm.
+          unfold transition_list in E. repeat dm. repeat inj_all.
+          unfold init_state in *. repeat dm. repeat inj_all.
+          assert(DFAaccepting (p, t, t0)
+                 = DFAaccepting (DFAtransition_list bs (p1, t3, t4))).
+          { rewrite E5. auto. }
+          rewrite H. clear H.
+          assert(DFAaccepting (p0, t1, t2)
+                 = DFAaccepting (regex2dfa (derivative_list bs e))).
+          { rewrite E. auto. }
+          rewrite H. clear H.
+          assert(DFAaccepting (DFAtransition_list bs (p1, t3, t4))
+                 = DFAaccepting (DFAtransition_list bs (regex2dfa e))).
+          { rewrite E2. auto. }
+          rewrite H. clear H.
+          apply DFAaccepting_dt_list.
+        Qed.
+        
+
+        Definition pointer_compare (s1 s2 : Pointer) : comparison :=
+          re_compare s1 s2.
+
+        Lemma pointer_compare_eq : forall x y,
+            pointer_compare x y = Eq <-> x = y.
+        Proof. apply re_compare_eq. Qed.
+
+        Lemma pointer_compare_trans : forall c x y z,
+            pointer_compare x y = c -> pointer_compare y z = c -> pointer_compare x z = c.
+        Proof. apply re_compare_trans. Qed.
+
+        Fixpoint pos2list (p : positive) : list bool :=
+          match p with
+          | xH => []
+          | xO p' => false :: (pos2list p')
+          | xI p' => true :: (pos2list p')
+          end.
+
+        Fixpoint list2pos (bs : list bool) : positive :=
+          match bs with
+          | [] => xH
+          | false :: bs' => xO (list2pos bs')
+          | true :: bs' => xI (list2pos bs')
+          end.
+
+        Lemma list_inv_pos : forall p,
+            list2pos (pos2list p) = p.
+        Proof.
+          induction p; sis; try rewrite IHp; auto.
+        Qed.
+
+        Definition int2list (z : Z) : list bool :=
+          match z with
+          | 0%Z => []
+          | Z.pos z' => true :: (pos2list z')
+          | Z.neg z' => false :: (pos2list z')
+          end.
+
+        Definition list2int (bs : list bool) : Z :=
+          match bs with
+          | [] => 0%Z
+          | true :: bs' => Z.pos (list2pos bs')
+          | false :: bs' => Z.neg (list2pos bs')
+          end.
+
+        Lemma list_inv_int : forall z,
+            list2int (int2list z) = z.
+        Proof.
+          destruct z.
+          - sis. auto.
+          - sis. rewrite list_inv_pos. auto.
+          - sis. rewrite list_inv_pos. auto.
+        Qed.
+
+        Definition index : Type := Z.
+        Definition index0 : index := 0%Z.
+
+        Lemma index_eq_dec : forall (i ii : index), {i = ii} + {i <> ii}.
+        Proof. repeat decide equality. Qed.
+        
+        Definition init_index (n : nat) : index :=
+          match n with
+          | 0 => index0
+          | S m => Z.pos (P_of_succ_nat m)
+          end.
+        
+        Definition index2list : index -> list bool:= int2list.
+        Definition list2index : list bool -> index := list2int.
+        
+        Lemma list_inv : forall (x : index), list2index (index2list x) = x.
+        Proof. apply list_inv_int. Qed.
+
+        Definition incr : index -> index := Z.succ.
+        Definition decr : index -> index := Z.pred.
+
+        (* for index correctness *)
+        Lemma decr_inv_incr : forall i, decr (incr i) = i.
+        Proof. apply Z.pred_succ. Qed.
+        
+        
+        Lemma incr_inv_decr : forall i, incr (decr i) = i.
+        Proof. apply Z.succ_pred. Qed.
+        
+        Lemma decr_inv_S : forall n, decr (init_index (S n)) = init_index n.
+        Proof.
+          induction n; auto.
+          sis. repeat dm.
+          - sis. inv E0.
+          - sis. inv E0. inv E. apply f_equal. rewrite H0. apply Pos.pred_double_succ.
+          - sis. inv E0.
+        Qed.
+        
+        Lemma incr_is_S : forall n, init_index (S n) = incr (init_index n).
+        Proof.
+          induction n; auto.
+          unfold init_index. unfold incr. apply Pos2Z.inj_succ.
+        Qed.
+        
+        Lemma n_det_index : forall n1 n2, init_index n1 = init_index n2 -> n1 = n2.
+        Proof.
+          intros. unfold init_index in *. destruct n1; destruct n2; try discriminate; auto.
+          repeat rewrite Znat.Zpos_P_of_succ_nat in H. repeat rewrite <- Znat.Nat2Z.inj_succ in *.
+          apply Znat.Nat2Z.inj; auto.
+        Qed.
+        
+      End Ty.
+      
+      Module Export Defs := state.DefsFn R Ty.
+
+    End STT.
+
+    Module Export MemTy <: MEMO STT := FMemo STT.
+
+    Module Export Defs := memo.MemoDefsFn STT MemTy.
+
+  End MEM.
 
   Module Import Correctness := memo.correctness.CorrectFn MEM.
 
@@ -28,8 +299,5 @@ Module LexerFn (ALPHABET : SIGMA) (LABELS : LABEL).
   Export R.Defs.
   Export STT.Defs.
   Export STT.R.Defs.
-  
 
 End LexerFn.
-
-  
